lib/coq/State_monad_lemmas.v
@@ -81,7 +81,7 @@ Require Export Morphisms Equivalence.
    equivalence for the state monad. *)
 Local Open Scope equiv_scope.
 #[export] Instance monadS_equivalence {Regs A E} :
-  Equivalence (pointwise_relation (sequential_state Regs) (@eq (list (result A E * sequential_state Regs)))) | 9.
+  Equivalence (pointwise_relation (sequential_state Regs) (pointwise_relation ChoiceSource (@eq (list (result A E * sequential_state Regs * ChoiceSource))))) | 9.
 split; apply _.
 Qed.
 
@@ -95,17 +95,17 @@ Qed.
 
 
 Lemma bindS_ext_cong (*[fundef_cong]:*) {Regs A B E}
-  {m1 m2 : monadS Regs A E} {f1 f2 : A -> monadS Regs B E} s :
-  m1 s = m2 s ->
-  (forall a s', List.In (Value a, s') (m2 s) -> f1 a s' = f2 a s') ->
-  bindS m1 f1 s = bindS m2 f2 s.
+  {m1 m2 : monadS Regs A E} {f1 f2 : A -> monadS Regs B E} s cs :
+  m1 s cs = m2 s cs ->
+  (forall a s' cs', List.In (Value a, s', cs') (m2 s cs) -> f1 a s' cs' = f2 a s' cs') ->
+  bindS m1 f1 s cs = bindS m2 f2 s cs.
 intros.
 unfold bindS.
 rewrite H.
 rewrite !List.flat_map_concat_map.
 f_equal.
 apply List.map_ext_in.
-intros [[a|a] s'] H_in; auto.
+intros [[[a|a] s'] cs'] H_in; auto.
 Qed.
 
 (* Weaker than the Isabelle version, but avoids talking about individual states *)
@@ -113,8 +113,9 @@ Lemma bindS_cong (*[fundef_cong]:*) Regs A B E m1 m2 (f1 f2 : A -> monadS Regs B
   m1 === m2 ->
   (forall a, f1 a === f2 a) ->
   bindS m1 f1 === bindS m2 f2.
-intros M F s.
+intros M F s cs.
 apply bindS_ext_cong; intros; auto.
+apply M.
 apply F.
 Qed.
 
@@ -125,7 +126,7 @@ Qed.
 
 Lemma bindS_returnS_left Regs A B E {x : A} {f : A -> monadS Regs B E} :
  bindS (returnS x) f === f x.
-intro s.
+intros s cs.
 unfold returnS, bindS.
 simpl.
 auto using List.app_nil_r.
@@ -135,9 +136,9 @@ Qed.
 
 Lemma bindS_returnS_right Regs A E {m : monadS Regs A E} :
  bindS m returnS === m.
-intro s.
+intros s cs.
 unfold returnS, bindS.
-induction (m s) as [|[[a|a] s'] t]; auto;
+induction (m s cs) as [|[[[a|a] s'] cs'] t]; auto;
 simpl;
 rewrite IHt;
 reflexivity.
@@ -145,16 +146,16 @@ Qed.
 #[export] Hint Rewrite bindS_returnS_right : state.
 #[export] Hint Resolve bindS_returnS_right : state.
 
-Lemma bindS_readS {Regs A E} {f} {m : A -> monadS Regs A E} {s} :
-  bindS (readS f) m s = m (f s) s.
+Lemma bindS_readS {Regs A E} {f} {m : A -> monadS Regs A E} {s cs} :
+  bindS (readS f) m s cs = m (f s) s cs.
 unfold readS, bindS.
 simpl.
 rewrite List.app_nil_r.
 reflexivity.
 Qed.
 
-Lemma bindS_updateS {Regs A E} {f : sequential_state Regs -> sequential_state Regs} {m : unit -> monadS Regs A E} {s} :
-  bindS (updateS f) m s = m tt (f s).
+Lemma bindS_updateS {Regs A E} {f : sequential_state Regs -> sequential_state Regs} {m : unit -> monadS Regs A E} {s cs} :
+  bindS (updateS f) m s cs = m tt (f s) cs.
 unfold updateS, bindS.
 simpl.
 auto using List.app_nil_r.
@@ -162,7 +163,7 @@ Qed.
 
 Lemma bindS_assertS_true Regs A E msg {f : unit -> monadS Regs A E} :
   bindS (assert_expS true msg) f === f tt.
-intro s.
+intros s cs.
 unfold assert_expS, bindS.
 simpl.
 auto using List.app_nil_r.
@@ -170,16 +171,16 @@ Qed.
 #[export] Hint Rewrite bindS_assertS_true : state.
 #[export] Hint Resolve bindS_assertS_true : state.
 
-Lemma bindS_chooseS_returnS (*[simp]:*) Regs A B E {xs : list A} {f : A -> B} :
-  bindS (Regs := Regs) (E := E) (chooseS xs) (fun x => returnS (f x)) === chooseS (List.map f xs).
-intro s.
+Lemma bindS_choose_listS_returnS (*[simp]:*) Regs A B E {xs : list A} {f : A -> B} :
+  bindS (Regs := Regs) (E := E) (choose_listS xs) (fun x => returnS (f x)) === choose_listS (List.map f xs).
+intros s cs.
 unfold chooseS, bindS, returnS.
 induction xs; auto.
 simpl. rewrite IHxs.
 reflexivity.
 Qed.
-#[export] Hint Rewrite bindS_chooseS_returnS : state.
-#[export] Hint Resolve bindS_chooseS_returnS : state.
+#[export] Hint Rewrite bindS_choose_listS_returnS : state.
+#[export] Hint Resolve bindS_choose_listS_returnS : state.
 
 Lemma result_cases : forall (A E : Type) (P : result A E -> Prop),
   (forall a, P (Value a)) ->
@@ -220,15 +221,15 @@ lemma monadS_eqI:
   using assms by (intro ext monadS_ext_eqI)
 *)
 
-Lemma bindS_cases {Regs A B E} {m} {f : A -> monadS Regs B E} {r s s'} :
-  List.In (r, s') (bindS m f s) ->
-  (exists a a' s'', r = Value a /\ List.In (Value a', s'') (m s) /\ List.In (Value a, s') (f a' s'')) \/
-  (exists e, r = Ex e /\ List.In (Ex e, s') (m s)) \/
-  (exists e a s'', r = Ex e /\ List.In (Value a, s'') (m s) /\ List.In (Ex e, s') (f a s'')).
+Lemma bindS_cases {Regs A B E} {m} {f : A -> monadS Regs B E} {r s s' cs cs'} :
+  List.In (r, s', cs') (bindS m f s cs) ->
+  (exists a a' s'' cs'', r = Value a /\ List.In (Value a', s'', cs'') (m s cs) /\ List.In (Value a, s', cs') (f a' s'' cs'')) \/
+  (exists e, r = Ex e /\ List.In (Ex e, s', cs') (m s cs)) \/
+  (exists e a s'' cs'', r = Ex e /\ List.In (Value a, s'', cs'') (m s cs) /\ List.In (Ex e, s', cs') (f a s'' cs'')).
 unfold bindS.
 intro IN.
 apply List.in_flat_map in IN.
-destruct IN as [[r' s''] [INr' INr]].
+destruct IN as [[[r' s''] cs''] [INr' INr]].
 destruct r' as [a'|e'].
 * destruct r as [a|e].
   + left. eauto 10.
@@ -236,21 +237,21 @@ destruct r' as [a'|e'].
 * right; left. simpl in INr. destruct INr as [|[]]. inversion H. subst. eauto 10.
 Qed.
 
-Lemma bindS_intro_Value {Regs A B E} {m} {f : A -> monadS Regs B E} {s a s' a' s''} :
- List.In (Value a', s'') (m s) -> List.In (Value a, s') (f a' s'') -> List.In (Value a, s') (bindS m f s).
+Lemma bindS_intro_Value {Regs A B E} {m} {f : A -> monadS Regs B E} {s cs a s' cs' a' s'' cs''} :
+ List.In (Value a', s'', cs'') (m s cs) -> List.In (Value a, s', cs') (f a' s'' cs'') -> List.In (Value a, s', cs') (bindS m f s cs).
 intros; unfold bindS.
 apply List.in_flat_map.
 eauto.
 Qed.
-Lemma bindS_intro_Ex_left {Regs A B E} {m} {f : A -> monadS Regs B E} {s e s'} :
-  List.In (Ex e, s') (m s) -> List.In (Ex e, s') (bindS m f s).
+Lemma bindS_intro_Ex_left {Regs A B E} {m} {f : A -> monadS Regs B E} {s cs e s' cs'} :
+  List.In (Ex e, s', cs') (m s cs) -> List.In (Ex e, s', cs') (bindS m f s cs).
 intros; unfold bindS.
 apply List.in_flat_map.
-exists (Ex e, s').
+exists (Ex e, s', cs').
 auto with datatypes.
 Qed.
-Lemma bindS_intro_Ex_right {Regs A B E} {m} {f : A -> monadS Regs B E} {s e s' a s''} :
-  List.In (Ex e, s') (f a s'') -> List.In (Value a, s'') (m s) -> List.In (Ex e, s') (bindS m f s).
+Lemma bindS_intro_Ex_right {Regs A B E} {m} {f : A -> monadS Regs B E} {s cs e s' cs' a s'' cs''} :
+  List.In (Ex e, s', cs') (f a s'' cs'') -> List.In (Value a, s'', cs'') (m s cs) -> List.In (Ex e, s', cs') (bindS m f s cs).
 intros; unfold bindS.
 apply List.in_flat_map.
 eauto.
@@ -259,9 +260,9 @@ Qed.
 
 Lemma bindS_assoc Regs A B C E {m} {f : A -> monadS Regs B E} {g : B -> monadS Regs C E} :
   bindS (bindS m f) g === bindS m (fun x => bindS (f x) g).
-intro s.
+intros s cs.
 unfold bindS.
-induction (m s) as [ | [[a | e] t]].
+induction (m s cs) as [ | [[[a | e] t] cs']].
 * reflexivity.
 * simpl. rewrite <- IHl.
   rewrite !List.flat_map_concat_map.
@@ -295,22 +296,22 @@ Qed.
 #[export] Hint Rewrite seqS_def : state.
 #[export] Hint Resolve seqS_def : state.
 
-Lemma Value_bindS_elim {Regs A B E} {a m} {f : A -> monadS Regs B E} {s s'} :
-  List.In (Value a, s') (bindS m f s) ->
-  exists s'' a', List.In (Value a', s'') (m s) /\ List.In (Value a, s') (f a' s'').
+Lemma Value_bindS_elim {Regs A B E} {a m} {f : A -> monadS Regs B E} {s cs s' cs'} :
+  List.In (Value a, s', cs') (bindS m f s cs) ->
+  exists s'' cs'' a', List.In (Value a', s'', cs'') (m s cs) /\ List.In (Value a, s', cs') (f a' s'' cs'').
 intro H.
 apply bindS_cases in H.
-destruct H as [(a0 & a' & s'' & [= <-] & [*]) | [(e & [= ] & _) | (_ & _ & _ & [= ] & _)]].
+destruct H as [(a0 & a' & s'' & cs'' & [= <-] & [*]) | [(e & [= ] & _) | (_ & _ & _ & _ & [= ] & _)]].
 eauto.
 Qed.
 
-Lemma Ex_bindS_elim {Regs A B E} {e m s s'} {f : A -> monadS Regs B E} :
-  List.In (Ex e, s') (bindS m f s) ->
-  List.In (Ex e, s') (m s) \/
-  exists s'' a', List.In (Value a', s'') (m s) /\ List.In (Ex e, s') (f a' s'').
+Lemma Ex_bindS_elim {Regs A B E} {e m s cs s' cs'} {f : A -> monadS Regs B E} :
+  List.In (Ex e, s', cs') (bindS m f s cs) ->
+  List.In (Ex e, s', cs') (m s cs) \/
+  exists s'' cs'' a', List.In (Value a', s'', cs'') (m s cs) /\ List.In (Ex e, s', cs') (f a' s'' cs'').
 intro H.
 apply bindS_cases in H.
-destruct H as [(? & ? & ? & [= ] & _) | [(? & [= <-] & X) | (? & ? & ? & [= <-] & X)]];
+destruct H as [(? & ? & ? & ? & [= ] & _) | [(? & [= <-] & X) | (? & ? & ? & ? & [= <-] & X)]];
 eauto.
 Qed.
 
@@ -328,7 +329,7 @@ Qed.
 #[export] Hint Resolve try_catchS_failS : state.
 Lemma try_catchS_throwS Regs A E1 E2 {e} {h : E1 -> monadS Regs A E2}:
   try_catchS (throwS e) h === h e.
-intro s.
+intros s cs.
 unfold try_catchS, throwS.
 simpl.
 auto using List.app_nil_r.
@@ -340,13 +341,13 @@ Lemma try_catchS_cong (*[cong]:*) {Regs A E1 E2 m1 m2} {h1 h2 : E1 -> monadS Reg
   m1 === m2 ->
   (forall e, h1 e === h2 e) ->
   try_catchS m1 h1 === try_catchS m2 h2.
-intros H1 H2 s.
+intros H1 H2 s cs.
 unfold try_catchS.
 rewrite H1.
 rewrite !List.flat_map_concat_map.
 f_equal.
 apply List.map_ext_in.
-intros [[a|[e|msg]] s'] H_in; auto. apply H2.
+intros [[[a|[e|msg]] s'] cs'] H_in; auto. apply H2.
 Qed.
 
 Add Parametric Morphism {Regs A E1 E2 : Type} : (@try_catchS Regs A E1 E2)
@@ -362,25 +363,25 @@ rewrite H.
 reflexivity.
 Qed.
 
-Lemma try_catchS_cases {Regs A E1 E2 m} {h : E1 -> monadS Regs A E2} {r s s'} :
-  List.In (r, s') (try_catchS m h s) ->
-  (exists a, r = Value a /\ List.In (Value a, s') (m s)) \/
-  (exists msg, r = Ex (Failure msg) /\ List.In (Ex (Failure msg), s') (m s)) \/
-  (exists e s'', List.In (Ex (Throw e), s'') (m s) /\ List.In (r, s') (h e s'')).
+Lemma try_catchS_cases {Regs A E1 E2 m} {h : E1 -> monadS Regs A E2} {r s cs s' cs'} :
+  List.In (r, s', cs') (try_catchS m h s cs) ->
+  (exists a, r = Value a /\ List.In (Value a, s', cs') (m s cs)) \/
+  (exists msg, r = Ex (Failure msg) /\ List.In (Ex (Failure msg), s', cs') (m s cs)) \/
+  (exists e s'' cs'', List.In (Ex (Throw e), s'', cs'') (m s cs) /\ List.In (r, s', cs') (h e s'' cs'')).
 unfold try_catchS.
 intro IN.
 apply List.in_flat_map in IN.
-destruct IN as [[r' s''] [INr' INr]].
+destruct IN as [[[r' s''] cs''] [INr' INr]].
 destruct r' as [a'|[e'|msg]].
-* left. simpl in INr. destruct INr as [[= <- <-] | []]. eauto 10.
-* simpl in INr. destruct INr as [[= <- <-] | []]. eauto 10.
+* left. simpl in INr. destruct INr as [[= <- <- <-] | []]. eauto 10.
+* simpl in INr. destruct INr as [[= <- <- <-] | []]. eauto 10.
 * eauto 10.
 Qed.
 
 Lemma try_catchS_intros {Regs A E1 E2} {m} {h : E1 -> monadS Regs A E2} :
-  (forall s a s', List.In (Value a, s') (m s) -> List.In (Value a, s') (try_catchS m h s)) /\
-  (forall s msg s', List.In (Ex (Failure msg), s') (m s) -> List.In (Ex (Failure msg), s') (try_catchS m h s)) /\
-  (forall s e s'' r s', List.In (Ex (Throw e), s'') (m s) -> List.In (r, s') (h e s'') -> List.In (r, s') (try_catchS m h s)).
+  (forall s cs a s' cs', List.In (Value a, s', cs') (m s cs) -> List.In (Value a, s', cs') (try_catchS m h s cs)) /\
+  (forall s cs msg s' cs', List.In (Ex (Failure msg), s', cs') (m s cs) -> List.In (Ex (Failure msg), s', cs') (try_catchS m h s cs)) /\
+  (forall s cs e s'' cs'' r s' cs', List.In (Ex (Throw e), s'', cs'') (m s cs) -> List.In (r, s', cs') (h e s'' cs'') -> List.In (r, s', cs') (try_catchS m h s cs)).
 repeat split; unfold try_catchS; intros;
 apply List.in_flat_map.
 * eexists; split; [ apply H | ]. simpl. auto.
@@ -388,11 +389,11 @@ apply List.in_flat_map.
 * eexists; split; [ apply H | ]. simpl. auto.
 Qed.
 
-Lemma no_Ex_basic_builtins (*[simp]:*) {Regs E} {s s' : sequential_state Regs} {e : ex E} :
-  (forall A (a:A), ~ List.In (Ex e, s') (returnS a s)) /\
-  (forall A (f : _ -> A), ~ List.In (Ex e, s') (readS f s)) /\
-  (forall f, ~ List.In (Ex e, s') (updateS f s)) /\
-  (forall A (xs : list A), ~ List.In (Ex e, s') (chooseS xs s)).
+Lemma no_Ex_basic_builtins (*[simp]:*) {Regs E} {s s' : sequential_state Regs} {cs cs'} {e : ex E} :
+  (forall A (a:A), ~ List.In (Ex e, s', cs') (returnS a s cs)) /\
+  (forall A (f : _ -> A), ~ List.In (Ex e, s', cs') (readS f s cs)) /\
+  (forall f, ~ List.In (Ex e, s', cs') (updateS f s cs)) /\
+  (forall A (xs : list A), ~ List.In (Ex e, s', cs') (choose_listS xs s cs)).
 repeat split; intros;
 unfold returnS, readS, updateS, chooseS; simpl;
 try intuition congruence.
@@ -403,37 +404,37 @@ try intuition congruence.
 Qed.
 
 Import List.ListNotations.
-Definition ignore_throw_aux {A E1 E2 S} (rs : result A E1 * S) : list (result A E2 * S) :=
+Definition ignore_throw_aux {A E1 E2 S CS} (rs : result A E1 * S * CS) : list (result A E2 * S * CS) :=
 match rs with
-| (Value a, s') => [(Value a, s')]
-| (Ex (Throw e), s') => []
-| (Ex (Failure msg), s') => [(Ex (Failure msg), s')]
+| (Value a, s', cs') => [(Value a, s', cs')]
+| (Ex (Throw e), s', cs') => []
+| (Ex (Failure msg), s', cs') => [(Ex (Failure msg), s', cs')]
 end.
-Definition ignore_throw {A E1 E2 S} (m : S -> list (result A E1 * S)) s : list (result A E2 * S) :=
- List.flat_map ignore_throw_aux (m s).
+Definition ignore_throw {A E1 E2 S CS} (m : S -> CS -> list (result A E1 * S * CS)) s cs : list (result A E2 * S * CS) :=
+ List.flat_map ignore_throw_aux (m s cs).
 
 Lemma ignore_throw_cong {Regs A E1 E2} {m1 m2 : monadS Regs A E1} :
   m1 === m2 ->
   ignore_throw (E2 := E2) m1 === ignore_throw m2.
-intros H s.
+intros H s cs.
 unfold ignore_throw.
 rewrite H.
 reflexivity.
 Qed.
 
-Lemma ignore_throw_aux_member_simps (*[simp]:*) {A E1 E2 S} {s' : S} {ms} :
-  (forall a:A, List.In (Value a, s') (ignore_throw_aux (E1 := E1) (E2 := E2) ms) <-> ms = (Value a, s')) /\
-  (forall e, ~ List.In (Ex (E := E2) (Throw e), s') (ignore_throw_aux ms)) /\
-  (forall msg, List.In (Ex (E := E2) (Failure msg), s') (ignore_throw_aux ms) <-> ms = (Ex (Failure msg), s')).
-destruct ms as [[a' | [e' | msg']] s]; simpl;
+Lemma ignore_throw_aux_member_simps (*[simp]:*) {A E1 E2 S CS} {s' : S} (cs' : CS) {ms} :
+  (forall a:A, List.In (Value a, s', cs') (ignore_throw_aux (E1 := E1) (E2 := E2) ms) <-> ms = (Value a, s', cs')) /\
+  (forall e, ~ List.In (Ex (E := E2) (Throw e), s', cs') (ignore_throw_aux ms)) /\
+  (forall msg, List.In (Ex (E := E2) (Failure msg), s', cs') (ignore_throw_aux ms) <-> ms = (Ex (Failure msg), s', cs')).
+destruct ms as [[[a' | [e' | msg']] s] cs]; simpl;
 intuition congruence.
 Qed.
 
-Lemma ignore_throw_member_simps (*[simp]:*) {A E1 E2 S} {s s' : S} {m} :
-  (forall {a:A}, List.In (Value (E := E2) a, s') (ignore_throw m s) <-> List.In (Value (E := E1) a, s') (m s)) /\
-  (forall {a:A}, List.In (Value (E := E2) a, s') (ignore_throw m s) <-> List.In (Value a, s') (m s)) /\
-  (forall e, ~ List.In (Ex (E := E2) (Throw e), s') (ignore_throw m s)) /\
-  (forall {msg}, List.In (Ex (E := E2) (Failure msg), s') (ignore_throw m s) <-> List.In (Ex (Failure msg), s') (m s)).
+Lemma ignore_throw_member_simps (*[simp]:*) {A E1 E2 S CS} {s s' : S} (cs cs' : CS) {m} :
+  (forall {a:A}, List.In (Value (E := E2) a, s', cs') (ignore_throw m s cs) <-> List.In (Value (E := E1) a, s', cs') (m s cs)) /\
+  (forall {a:A}, List.In (Value (E := E2) a, s', cs') (ignore_throw m s cs) <-> List.In (Value a, s', cs') (m s cs)) /\
+  (forall e, ~ List.In (Ex (E := E2) (Throw e), s', cs') (ignore_throw m s cs)) /\
+  (forall {msg}, List.In (Ex (E := E2) (Failure msg), s', cs') (ignore_throw m s cs) <-> List.In (Ex (Failure msg), s', cs') (m s cs)).
 unfold ignore_throw.
 repeat apply conj; intros; try apply conj;
 rewrite ?List.in_flat_map;
@@ -442,9 +443,9 @@ solve
 | intro H; eexists; split; [ apply H | apply ignore_throw_aux_member_simps; reflexivity] ].
 Qed.
 
-Lemma ignore_throw_cases {A E S} {m : S -> list (result A E * S)} {r s s'} :
-  ignore_throw m s = m s ->
-  List.In (r, s') (m s) ->
+Lemma ignore_throw_cases {A E S CS} {m : S -> CS -> list (result A E * S * CS)} {r s cs s' cs'} :
+  ignore_throw m s cs = m s cs ->
+  List.In (r, s', cs') (m s cs) ->
   (exists a, r = Value a) \/
   (exists msg, r = Ex (Failure msg)).
 destruct r as [a | [e | msg]]; eauto.
@@ -463,9 +464,9 @@ Qed.
 
 Lemma ignore_throw_bindS (*[simp]:*) Regs A B E E2 {m} {f : A -> monadS Regs B E} :
   ignore_throw (E2 := E2) (bindS m f) === bindS (ignore_throw m) (fun s => ignore_throw (f s)).
-intro s.
+intros s cs.
 unfold bindS, ignore_throw.
-induction (m s) as [ | [[a | [e | msg]] t]].
+induction (m s cs) as [ | [[[a | [e | msg]] t] cs']].
 * reflexivity.
 * simpl. rewrite <- IHl. rewrite flat_map_app. reflexivity.
 * simpl. rewrite <- IHl. reflexivity.
@@ -480,14 +481,14 @@ Lemma try_catchS_bindS_no_throw {Regs A B E1 E2} {m1 : monadS Regs A E1} {m2 : m
   try_catchS (bindS m1 f) h === bindS m2 (fun a => try_catchS (f a) h).
 intros Ignore1 Ignore2.
 transitivity ((ignore_throw m1 >>$= (fun a => try_catchS (f a) h))).
-* intro s.
+* intros s cs.
   unfold bindS, try_catchS, ignore_throw.
-  specialize (Ignore1 s). revert Ignore1. unfold ignore_throw.
-  induction (m1 s) as [ | [[a | [e | msg]] t]]; auto.
+  specialize (Ignore1 s cs). revert Ignore1. unfold ignore_throw.
+  induction (m1 s cs) as [ | [[[a | [e | msg]] t] cs']]; auto.
   + intro Ig. simpl. rewrite flat_map_app. rewrite IHl. auto. injection Ig. auto.
   + intro Ig. simpl. rewrite IHl. reflexivity. injection Ig. auto.
   + intro Ig. exfalso. clear -Ig.
-    assert (List.In (Ex (Throw msg), t) (List.flat_map ignore_throw_aux l)).
+    assert (List.In (Ex (Throw msg), t, cs') (List.flat_map ignore_throw_aux l)).
     simpl in Ig. rewrite Ig. simpl. auto.
     apply List.in_flat_map in H.
     destruct H as [x [H1 H2]].
@@ -512,16 +513,19 @@ Lemma no_throw_basic_builtins_3 Regs E E2 {f : sequential_state Regs -> sequenti
   ignore_throw (E1 := E) (E2 := E2) (updateS f) = updateS f.
 reflexivity. Qed.
 Lemma no_throw_basic_builtins_4 Regs A E1 E2 {xs : list A} :
-  ignore_throw (E1 := E1) (chooseS xs) === @chooseS Regs A E2 xs.
-intro s.
-unfold ignore_throw, chooseS.
+  ignore_throw (E1 := E1) (choose_listS xs) === @choose_listS Regs A E2 xs.
+intros s cs.
+unfold ignore_throw, choose_listS.
 rewrite List.flat_map_concat_map, List.map_map. simpl.
 rewrite concat_map_singleton.
 reflexivity.
 Qed.
-Lemma no_throw_basic_builtins_5 Regs E1 E2 :
-  ignore_throw (E1 := E1) (choose_boolS tt) = @choose_boolS Regs E2 tt.
-reflexivity. Qed.
+Lemma no_throw_basic_builtins_5 Regs E1 E2 ty :
+  ignore_throw (E1 := E1) (chooseS ty) === @chooseS Regs E2 ty.
+intros s cs.
+unfold ignore_throw, chooseS.
+destruct (choose cs ty); reflexivity.
+Qed.
 Lemma no_throw_basic_builtins_6 Regs A E1 E2 msg :
   ignore_throw (E1 := E1) (failS msg) = @failS Regs A E2 msg.
 reflexivity. Qed.
@@ -622,12 +626,13 @@ Lemma no_throw_mem_builtins_10 Regs E1 E2 :
 reflexivity. Qed.
 #[export] Hint Rewrite no_throw_mem_builtins_10 : ignore_throw.
 #[export] Hint Resolve no_throw_mem_builtins_10 : ignore_throw.
+(*
 Lemma no_throw_mem_builtins_11 Regs E1 E2 :
   ignore_throw (E2 := E2) (@undefined_boolS Regs E1 tt) === undefined_boolS tt.
 reflexivity. Qed.
 #[export] Hint Rewrite no_throw_mem_builtins_11 : ignore_throw.
 #[export] Hint Resolve no_throw_mem_builtins_11 : ignore_throw.
-
+*)
 Lemma no_throw_read_regvalS Regs RV E1 E2 r reg_name :
   ignore_throw (E2 := E2) (@read_regvalS Regs RV E1 r reg_name) === read_regvalS r reg_name.
 destruct r; simpl. autorewrite with ignore_throw.
